Refactor

src/verification/vars.lean
@@ -45,18 +45,17 @@ inductive Types
 section Ident
 
 @[derive decidable_eq]
-structure Ident :=
+structure Ident (b : Types) :=
 (ns : NameSpace)
 (name : Vars)
-(type : Types)
 
-instance : has_to_string Ident :=
+instance {b : Types} : has_to_string (Ident b) :=
 ⟨λ i, "n" ++ (to_string i.ns) ++ "_" ++ (to_string i.name)⟩
 
-lemma Ident_ns_surjective : function.surjective Ident.ns :=
-by { intro x, use ⟨x, default, default⟩, }
+lemma Ident_ns_surjective {b : Types} : function.surjective (@Ident.ns b) :=
+by { intro x, use ⟨x, default⟩, }
 
-@[simp] lemma Ident_ns_range : set.range Ident.ns = set.univ :=
+@[simp] lemma Ident_ns_range {b : Types} : set.range (@Ident.ns b) = set.univ :=
 by simpa [set.surjective_iff_surj_on_univ, set.surj_on, set.univ_subset_iff] using Ident_ns_surjective
 
 local infix `∷`:9000 := Ident.mk
@@ -64,6 +63,7 @@ local infix `∷`:9000 := Ident.mk
 end Ident
 
 section frames
+-- TODO Fix
 variables {α γ : Type*} {β : α → Type*} (f : (Π x, β x) → γ) (g : (Π x, β x) → (Π x, β x))
 
 def function.has_dframe (S : set α) : Prop :=
@@ -73,9 +73,20 @@ structure function.has_dheap (S : set α) : Prop :=
 (local_frame : ∀ (c₁ c₂ : Π x, β x), (∀ x ∈ S, c₁ x = c₂ x) → ∀ {y}, y ∈ S → g c₁ y = g c₂ y)
 (global_id : ∀ (c y), y ∉ S → g c y = c y)
 
-theorem function.has_dframe.res {S S'} (h : function.has_dframe f S) (hS' : S ⊆ S') :
+variables {f g}
+theorem function.has_dframe.res {S} (h : function.has_dframe f S) (S') (hS' : S ⊆ S') :
   function.has_dframe f S' :=
 λ c₁ c₂ h', h (λ x hx, h' _ (hS' hx))
+
+theorem function.has_dheap.res {S} (h : function.has_dheap g S) (S') (hS' : S ⊆ S') :
+  function.has_dheap g S' :=
+{ local_frame := λ c₁ c₂ c_eq y hy, 
+begin
+  by_cases H : y ∈ S,
+  { exact h.local_frame c₁ c₂ (λ x hx, c_eq _ (hS' hx)) H, },
+  { rw [h.global_id c₁ _ H, h.global_id c₂ _ H],  exact c_eq _ hy, },
+end,
+  global_id := λ c y hy, h.global_id c y (λ H, hy (hS' H)), }
 
 theorem function.has_dframe.const (x : γ) (S : set α) : function.has_dframe (λ _ : Π x, β x, x) S :=
 λ _ _ _, rfl
@@ -84,4 +95,18 @@ theorem function.has_dheap.id (S : set α) : function.has_dheap (@id (Π x, β x
 { local_frame := λ c₁ c₂ h y hy, h y hy,
   global_id := λ _ _ _, rfl }
 
+example {S : set α} {x₀ : α} {y₀ : β x₀} [∀ x, decidable_eq (β x)] (f : (Π x, β x) → (Π x, β x)) (g : (Π x, β x) → γ)
+  (hf : function.has_dframe g S) (hg : function.has_dheap f (insert x₀ S)) :
+  function.has_dframe (λ ctx, if ctx x₀ = y₀ then g (f ctx) else g ctx) (insert x₀ S) :=
+begin
+  intros c₁ c₂ c_eq, dsimp only,
+  have := (hf.res _ _) c_eq,
+  all_goals { sorry, },
+end
+
 end frames
+
+section iterate
+
+def iterate_while {α : Type*} (f : α → α) (cond : α → Prop) [decidable_pred cond] : ℕ → α → α := sorry
+end iterate
